Beautifying an old entry

src/HOL/Induct/PropLog.thy
@@ -14,28 +14,28 @@ text \<open>
   Inductive definition of propositional logic.  Soundness and
   completeness w.r.t.\ truth-tables.
 
-  Prove: If \<open>H |= p\<close> then \<open>G |= p\<close> where \<open>G \<in>
+  Prove: If \<open>H \<Turnstile> p\<close> then \<open>G \<Turnstile> p\<close> where \<open>G \<in>
   Fin(H)\<close>
 \<close>
 
 subsection \<open>The datatype of propositions\<close>
 
 datatype 'a pl =
-  false |
-  var 'a ("#_" [1000]) |
-  imp "'a pl" "'a pl" (infixr "->" 90)
+    false 
+  | var 'a ("#_" [1000]) 
+  | imp "'a pl" "'a pl" (infixr "\<rightharpoonup>" 90)
 
 
 subsection \<open>The proof system\<close>
 
-inductive thms :: "['a pl set, 'a pl] => bool"  (infixl "|-" 50)
+inductive thms :: "['a pl set, 'a pl] \<Rightarrow> bool"  (infixl "\<turnstile>" 50)
   for H :: "'a pl set"
-where
-  H: "p\<in>H ==> H |- p"
-| K: "H |- p->q->p"
-| S: "H |- (p->q->r) -> (p->q) -> p->r"
-| DN: "H |- ((p->false) -> false) -> p"
-| MP: "[| H |- p->q; H |- p |] ==> H |- q"
+  where
+    H: "p \<in> H \<Longrightarrow> H \<turnstile> p"
+  | K: "H \<turnstile> p\<rightharpoonup>q\<rightharpoonup>p"
+  | S: "H \<turnstile> (p\<rightharpoonup>q\<rightharpoonup>r) \<rightharpoonup> (p\<rightharpoonup>q) \<rightharpoonup> p\<rightharpoonup>r"
+  | DN: "H \<turnstile> ((p\<rightharpoonup>false) \<rightharpoonup> false) \<rightharpoonup> p"
+  | MP: "\<lbrakk>H \<turnstile> p\<rightharpoonup>q; H \<turnstile> p\<rbrakk> \<Longrightarrow> H \<turnstile> q"
 
 
 subsection \<open>The semantics\<close>
@@ -43,10 +43,10 @@ subsection \<open>The semantics\<close>
 subsubsection \<open>Semantics of propositional logic.\<close>
 
 primrec eval :: "['a set, 'a pl] => bool"  ("_[[_]]" [100,0] 100)
-where
-  "tt[[false]] = False"
-| "tt[[#v]] = (v \<in> tt)"
-| eval_imp: "tt[[p->q]] = (tt[[p]] --> tt[[q]])"
+  where
+    "tt[[false]] = False"
+  | "tt[[#v]] = (v \<in> tt)"
+  | eval_imp: "tt[[p\<rightharpoonup>q]] = (tt[[p]] \<longrightarrow> tt[[q]])"
 
 text \<open>
   A finite set of hypotheses from \<open>t\<close> and the \<open>Var\<close>s in
@@ -54,10 +54,10 @@ text \<open>
 \<close>
 
 primrec hyps :: "['a pl, 'a set] => 'a pl set"
-where
-  "hyps false  tt = {}"
-| "hyps (#v)   tt = {if v \<in> tt then #v else #v->false}"
-| "hyps (p->q) tt = hyps p tt Un hyps q tt"
+  where
+    "hyps false  tt = {}"
+  | "hyps (#v)   tt = {if v \<in> tt then #v else #v\<rightharpoonup>false}"
+  | "hyps (p\<rightharpoonup>q) tt = hyps p tt Un hyps q tt"
 
 
 subsubsection \<open>Logical consequence\<close>
@@ -67,98 +67,97 @@ text \<open>
   is \<open>p\<close>.
 \<close>
 
-definition sat :: "['a pl set, 'a pl] => bool"  (infixl "|=" 50)
-  where "H |= p = (\<forall>tt. (\<forall>q\<in>H. tt[[q]]) --> tt[[p]])"
+definition sat :: "['a pl set, 'a pl] => bool"  (infixl "\<Turnstile>" 50)
+  where "H \<Turnstile> p = (\<forall>tt. (\<forall>q\<in>H. tt[[q]]) \<longrightarrow> tt[[p]])"
 
 
 subsection \<open>Proof theory of propositional logic\<close>
 
-lemma thms_mono: "G<=H ==> thms(G) <= thms(H)"
-apply (rule predicate1I)
-apply (erule thms.induct)
-apply (auto intro: thms.intros)
-done
+lemma thms_mono: 
+  assumes "G \<subseteq> H" shows "thms(G) \<le> thms(H)"
+proof -
+  have "G \<turnstile> p \<Longrightarrow> H \<turnstile> p" for p
+    by (induction rule: thms.induct) (use assms in \<open>auto intro: thms.intros\<close>)
+  then show ?thesis
+    by blast
+qed
 
-lemma thms_I: "H |- p->p"
+lemma thms_I: "H \<turnstile> p\<rightharpoonup>p"
   \<comment> \<open>Called \<open>I\<close> for Identity Combinator, not for Introduction.\<close>
-by (best intro: thms.K thms.S thms.MP)
+  by (best intro: thms.K thms.S thms.MP)
 
 
 subsubsection \<open>Weakening, left and right\<close>
 
-lemma weaken_left: "[| G \<subseteq> H;  G|-p |] ==> H|-p"
+lemma weaken_left: "\<lbrakk>G \<subseteq> H;  G\<turnstile>p\<rbrakk> \<Longrightarrow> H\<turnstile>p"
   \<comment> \<open>Order of premises is convenient with \<open>THEN\<close>\<close>
-  by (erule thms_mono [THEN predicate1D])
+  by (meson predicate1D thms_mono)
 
-lemma weaken_left_insert: "G |- p \<Longrightarrow> insert a G |- p"
-by (rule weaken_left) (rule subset_insertI)
+lemma weaken_left_insert: "G \<turnstile> p \<Longrightarrow> insert a G \<turnstile> p"
+  by (meson subset_insertI weaken_left)
 
-lemma weaken_left_Un1: "G |- p \<Longrightarrow> G \<union> B |- p"
-by (rule weaken_left) (rule Un_upper1)
+lemma weaken_left_Un1: "G \<turnstile> p \<Longrightarrow> G \<union> B \<turnstile> p"
+  by (rule weaken_left) (rule Un_upper1)
 
-lemma weaken_left_Un2: "G |- p \<Longrightarrow> A \<union> G |- p"
-by (rule weaken_left) (rule Un_upper2)
+lemma weaken_left_Un2: "G \<turnstile> p \<Longrightarrow> A \<union> G \<turnstile> p"
+  by (metis Un_commute weaken_left_Un1)
 
-lemma weaken_right: "H |- q ==> H |- p->q"
-by (fast intro: thms.K thms.MP)
+lemma weaken_right: "H \<turnstile> q \<Longrightarrow> H \<turnstile> p\<rightharpoonup>q"
+  using K MP by blast
 
 
 subsubsection \<open>The deduction theorem\<close>
 
-theorem deduction: "insert p H |- q  ==>  H |- p->q"
-apply (induct set: thms)
-apply (fast intro: thms_I thms.H thms.K thms.S thms.DN
-                   thms.S [THEN thms.MP, THEN thms.MP] weaken_right)+
-done
+theorem deduction: "insert p H \<turnstile> q  \<Longrightarrow>  H \<turnstile> p\<rightharpoonup>q"
+proof (induct set: thms)
+  case (H p)
+  then show ?case
+    using thms.H thms_I weaken_right by fastforce 
+qed (metis thms.simps)+
 
 
 subsubsection \<open>The cut rule\<close>
 
-lemma cut: "insert p H |- q \<Longrightarrow> H |- p \<Longrightarrow> H |- q"
-by (rule thms.MP) (rule deduction)
+lemma cut: "insert p H \<turnstile> q \<Longrightarrow> H \<turnstile> p \<Longrightarrow> H \<turnstile> q"
+  using MP deduction by blast
 
-lemma thms_falseE: "H |- false \<Longrightarrow> H |- q"
-by (rule thms.MP, rule thms.DN) (rule weaken_right)
+lemma thms_falseE: "H \<turnstile> false \<Longrightarrow> H \<turnstile> q"
+  by (metis thms.simps)
 
-lemma thms_notE: "H |- p -> false \<Longrightarrow> H |- p \<Longrightarrow> H |- q"
-by (rule thms_falseE) (rule thms.MP)
+lemma thms_notE: "H \<turnstile> p \<rightharpoonup> false \<Longrightarrow> H \<turnstile> p \<Longrightarrow> H \<turnstile> q"
+  using MP thms_falseE by blast
 
 
 subsubsection \<open>Soundness of the rules wrt truth-table semantics\<close>
 
-theorem soundness: "H |- p ==> H |= p"
-by (induct set: thms) (auto simp: sat_def)
+theorem soundness: "H \<turnstile> p \<Longrightarrow> H \<Turnstile> p"
+  by (induct set: thms) (auto simp: sat_def)
 
 
 subsection \<open>Completeness\<close>
 
 subsubsection \<open>Towards the completeness proof\<close>
 
-lemma false_imp: "H |- p->false ==> H |- p->q"
-apply (rule deduction)
-apply (metis H insert_iff weaken_left_insert thms_notE)
-done
+lemma false_imp: "H \<turnstile> p\<rightharpoonup>false \<Longrightarrow> H \<turnstile> p\<rightharpoonup>q"
+  by (metis thms.simps)
 
 lemma imp_false:
-    "[| H |- p;  H |- q->false |] ==> H |- (p->q)->false"
-apply (rule deduction)
-apply (metis H MP insert_iff weaken_left_insert)
-done
+  "\<lbrakk>H \<turnstile> p;  H \<turnstile> q\<rightharpoonup>false\<rbrakk> \<Longrightarrow> H \<turnstile> (p\<rightharpoonup>q)\<rightharpoonup>false"
+  by (meson MP S weaken_right)
 
-lemma hyps_thms_if: "hyps p tt |- (if tt[[p]] then p else p->false)"
+lemma hyps_thms_if: "hyps p tt \<turnstile> (if tt[[p]] then p else p\<rightharpoonup>false)"
   \<comment> \<open>Typical example of strengthening the induction statement.\<close>
-apply simp
-apply (induct p)
-apply (simp_all add: thms_I thms.H)
-apply (blast intro: weaken_left_Un1 weaken_left_Un2 weaken_right
-                    imp_false false_imp)
-done
+proof (induction p)
+  case (imp p1 p2)
+  then show ?case
+    by (metis (full_types) eval_imp false_imp hyps.simps(3) imp_false weaken_left_Un1 weaken_left_Un2 weaken_right)
 
-lemma sat_thms_p: "{} |= p ==> hyps p tt |- p"
+qed (simp_all add: thms_I thms.H)
+
+lemma sat_thms_p: "{} \<Turnstile> p \<Longrightarrow> hyps p tt \<turnstile> p"
   \<comment> \<open>Key lemma for completeness; yields a set of assumptions
         satisfying \<open>p\<close>\<close>
-unfolding sat_def
-by (metis (full_types) empty_iff hyps_thms_if)
+  by (metis (full_types) empty_iff hyps_thms_if sat_def)
 
 text \<open>
   For proving certain theorems in our new propositional logic.
@@ -171,54 +170,57 @@ text \<open>
   The excluded middle in the form of an elimination rule.
 \<close>
 
-lemma thms_excluded_middle: "H |- (p->q) -> ((p->false)->q) -> q"
-apply (rule deduction [THEN deduction])
-apply (rule thms.DN [THEN thms.MP], best intro: H)
-done
+lemma thms_excluded_middle: "H \<turnstile> (p\<rightharpoonup>q) \<rightharpoonup> ((p\<rightharpoonup>false)\<rightharpoonup>q) \<rightharpoonup> q"
+proof -
+  have "insert ((p \<rightharpoonup> false) \<rightharpoonup> q) (insert (p \<rightharpoonup> q) H) \<turnstile> (q \<rightharpoonup> false) \<rightharpoonup> false"
+    by (best intro: H)
+  then show ?thesis
+    by (metis deduction thms.simps)
+qed
 
 lemma thms_excluded_middle_rule:
-    "[| insert p H |- q;  insert (p->false) H |- q |] ==> H |- q"
+  "\<lbrakk>insert p H \<turnstile> q;  insert (p\<rightharpoonup>false) H \<turnstile> q\<rbrakk> \<Longrightarrow> H \<turnstile> q"
   \<comment> \<open>Hard to prove directly because it requires cuts\<close>
-by (rule thms_excluded_middle [THEN thms.MP, THEN thms.MP], auto)
+  by (rule thms_excluded_middle [THEN thms.MP, THEN thms.MP], auto)
 
 
 subsection\<open>Completeness -- lemmas for reducing the set of assumptions\<close>
 
 text \<open>
-  For the case \<^prop>\<open>hyps p t - insert #v Y |- p\<close> we also have \<^prop>\<open>hyps p t - {#v} \<subseteq> hyps p (t-{v})\<close>.
+  For the case \<^prop>\<open>hyps p t - insert #v Y \<turnstile> p\<close> we also have \<^prop>\<open>hyps p t - {#v} \<subseteq> hyps p (t-{v})\<close>.
 \<close>
 
-lemma hyps_Diff: "hyps p (t-{v}) <= insert (#v->false) ((hyps p t)-{#v})"
-by (induct p) auto
+lemma hyps_Diff: "hyps p (t-{v}) \<subseteq> insert (#v\<rightharpoonup>false) ((hyps p t)-{#v})"
+  by (induct p) auto
 
 text \<open>
-  For the case \<^prop>\<open>hyps p t - insert (#v -> Fls) Y |- p\<close> we also have
-  \<^prop>\<open>hyps p t-{#v->Fls} \<subseteq> hyps p (insert v t)\<close>.
+  For the case \<^prop>\<open>hyps p t - insert (#v \<rightharpoonup> Fls) Y \<turnstile> p\<close> we also have
+  \<^prop>\<open>hyps p t-{#v\<rightharpoonup>Fls} \<subseteq> hyps p (insert v t)\<close>.
 \<close>
 
-lemma hyps_insert: "hyps p (insert v t) <= insert (#v) (hyps p t-{#v->false})"
-by (induct p) auto
+lemma hyps_insert: "hyps p (insert v t) \<subseteq> insert (#v) (hyps p t-{#v\<rightharpoonup>false})"
+  by (induct p) auto
 
 text \<open>Two lemmas for use with \<open>weaken_left\<close>\<close>
 
-lemma insert_Diff_same: "B-C <= insert a (B-insert a C)"
-by fast
+lemma insert_Diff_same: "B-C \<subseteq> insert a (B-insert a C)"
+  by fast
 
-lemma insert_Diff_subset2: "insert a (B-{c}) - D <= insert a (B-insert c D)"
-by fast
+lemma insert_Diff_subset2: "insert a (B-{c}) - D \<subseteq> insert a (B-insert c D)"
+  by fast
 
 text \<open>
   The set \<^term>\<open>hyps p t\<close> is finite, and elements have the form
-  \<^term>\<open>#v\<close> or \<^term>\<open>#v->Fls\<close>.
+  \<^term>\<open>#v\<close> or \<^term>\<open>#v\<rightharpoonup>Fls\<close>.
 \<close>
 
 lemma hyps_finite: "finite(hyps p t)"
-by (induct p) auto
+  by (induct p) auto
 
-lemma hyps_subset: "hyps p t <= (UN v. {#v, #v->false})"
-by (induct p) auto
+lemma hyps_subset: "hyps p t \<subseteq> (UN v. {#v, #v\<rightharpoonup>false})"
+  by (induct p) auto
 
-lemma Diff_weaken_left: "A \<subseteq> C \<Longrightarrow> A - B |- p \<Longrightarrow> C - B |- p"
+lemma Diff_weaken_left: "A \<subseteq> C \<Longrightarrow> A - B \<turnstile> p \<Longrightarrow> C - B \<turnstile> p"
   by (rule Diff_mono [OF _ subset_refl, THEN weaken_left])
 
 
@@ -229,37 +231,55 @@ text \<open>
   may repeatedly subtract assumptions until none are left!
 \<close>
 
-lemma completeness_0_lemma:
-    "{} |= p ==> \<forall>t. hyps p t - hyps p t0 |- p"
-apply (rule hyps_subset [THEN hyps_finite [THEN finite_subset_induct]])
- apply (simp add: sat_thms_p, safe)
- txt\<open>Case \<open>hyps p t-insert(#v,Y) |- p\<close>\<close>
- apply (iprover intro: thms_excluded_middle_rule
-                     insert_Diff_same [THEN weaken_left]
-                     insert_Diff_subset2 [THEN weaken_left]
-                     hyps_Diff [THEN Diff_weaken_left])
-txt\<open>Case \<open>hyps p t-insert(#v -> false,Y) |- p\<close>\<close>
- apply (iprover intro: thms_excluded_middle_rule
-                     insert_Diff_same [THEN weaken_left]
-                     insert_Diff_subset2 [THEN weaken_left]
-                     hyps_insert [THEN Diff_weaken_left])
-done
-
-text\<open>The base case for completeness\<close>
-lemma completeness_0:  "{} |= p ==> {} |- p"
-  by (metis Diff_cancel completeness_0_lemma)
+lemma completeness_0: 
+  assumes "{} \<Turnstile> p"
+  shows "{} \<turnstile> p"
+proof -
+  { fix t t0
+    have "hyps p t - hyps p t0 \<turnstile> p"
+      using hyps_finite hyps_subset
+    proof (induction arbitrary: t rule: finite_subset_induct)
+      case empty
+      then show ?case
+        by (simp add: assms sat_thms_p)
+    next
+      case (insert q H)
+      then consider v where "q = #v" | v where "q = #v \<rightharpoonup> false"
+        by blast
+      then show ?case
+      proof cases
+        case 1
+        then show ?thesis
+          by (metis (no_types, lifting) insert.IH thms_excluded_middle_rule insert_Diff_same 
+              insert_Diff_subset2 weaken_left Diff_weaken_left hyps_Diff)
+      next
+        case 2
+        then show ?thesis
+          by (metis (no_types, lifting) insert.IH thms_excluded_middle_rule insert_Diff_same 
+              insert_Diff_subset2 weaken_left Diff_weaken_left hyps_insert)
+      qed
+    qed
+  }
+  then show ?thesis
+    by (metis Diff_cancel)
+qed
 
 text\<open>A semantic analogue of the Deduction Theorem\<close>
-lemma sat_imp: "insert p H |= q ==> H |= p->q"
-by (auto simp: sat_def)
+lemma sat_imp: "insert p H \<Turnstile> q \<Longrightarrow> H \<Turnstile> p\<rightharpoonup>q"
+  by (auto simp: sat_def)
 
-theorem completeness: "finite H ==> H |= p ==> H |- p"
-apply (induct arbitrary: p rule: finite_induct)
- apply (blast intro: completeness_0)
-apply (iprover intro: sat_imp thms.H insertI1 weaken_left_insert [THEN thms.MP])
-done
+theorem completeness: "finite H \<Longrightarrow> H \<Turnstile> p \<Longrightarrow> H \<turnstile> p"
+proof (induction arbitrary: p rule: finite_induct)
+  case empty
+  then show ?case
+    by (simp add: completeness_0)
+next
+  case insert
+  then show ?case
+    by (meson H MP insertI1 sat_imp weaken_left_insert)
+qed
 
-theorem syntax_iff_semantics: "finite H ==> (H |- p) = (H |= p)"
-by (blast intro: soundness completeness)
+theorem syntax_iff_semantics: "finite H \<Longrightarrow> (H \<turnstile> p) = (H \<Turnstile> p)"
+  by (blast intro: soundness completeness)
 
 end
